update

Communication_Topology_Analysis.thy
@@ -81,8 +81,8 @@ inductive exp_reachable :: "abstract_value_env \<times> exp \<Rightarrow> exp \<
   " |
   Let: "
     \<lbrakk>
-     (\<V>, e) \<downharpoonright> (LET x = b in e');
-     ^\<omega> \<in> \<V> x
+      (\<V>, e) \<downharpoonright> (LET x = b in e');
+      ^\<omega> \<in> \<V> x
     \<rbrakk> \<Longrightarrow>
     (\<V>, e) \<downharpoonright> e'
   " |
@@ -114,6 +114,18 @@ inductive exp_reachable :: "abstract_value_env \<times> exp \<Rightarrow> exp \<
     (\<V>, e) \<downharpoonright> e\<^sub>c
   "
 
+inductive pool_reachable :: "abstract_value_env \<times> state_pool \<Rightarrow> state_pool \<Rightarrow> bool" (infix "\<downharpoonright>\<downharpoonright>" 55) where
+  Any: "
+    \<lbrakk>
+      \<forall> \<pi>' e' \<rho>' \<kappa>' . \<E>' \<pi>' = Some (\<langle>e';\<rho>';\<kappa>'\<rangle>) \<longrightarrow>
+        (\<exists> \<pi> e \<rho> \<kappa> . 
+          \<E> \<pi> = Some (\<langle>e;\<rho>;\<kappa>\<rangle>) \<and>
+          prefix \<pi> \<pi>' \<and> leaf \<E> \<pi> \<and>
+          (\<V>, e) \<downharpoonright> e'
+        )
+    \<rbrakk> \<Longrightarrow>
+    (\<V>, \<E>) \<downharpoonright>\<downharpoonright> \<E>'
+  "
 
 inductive path_reachable :: "abstract_value_env \<times> exp \<Rightarrow> control_path \<Rightarrow> bool" (infix ":\<downharpoonright>" 55) where
   Empty: "
